theories/Equiv/BisimEq.v
@@ -1,0 +1,135 @@
+Require Import Util MapDefined LengthEq Map CSet AutoIndTac AllInRel.
+Require Import Var Val Exp Envs IL SimF.
+
+Set Implicit Arguments.
+Unset Printing Records.
+
+(** * Program Equivalence *)
+
+Instance SR : PointwiseProofRelationF (nat) := {
+   ParamRelFP G Z Z' := ❬Z❭ = ❬Z'❭ /\ ❬Z❭ = G;
+   ArgRelFP E E' G VL VL' := VL = VL' /\ length VL = G;
+}.
+
+Definition bisimeq r t s s' :=
+    forall L L' E, labenv_sim t (sim r) SR (@length _ ⊝ F.block_Z ⊝ L') L L'
+            -> ❬L❭ = ❬L'❭
+            -> sim r t (L:F.labenv, E, s) (L', E, s').
+
+(** ** Reflexivity *)
+
+Lemma bisimeq_refl s t
+  : forall L L' E r,
+    labenv_sim t (sim r) SR (@length _ ⊝ block_Z ⊝ L') L L'
+    -> sim r t (L, E, s) (L', E, s).
+Proof.
+  sind s; destruct s; simpl in *; intros.
+  - destruct e.
+    + eapply (sim_let_op il_statetype_F); eauto.
+    + eapply (sim_let_call il_statetype_F); eauto.
+  - eapply (sim_cond il_statetype_F); eauto.
+  - edestruct (get_dec L' (counted l)) as [[b]|]; [ inv_get | ].
+    + eapply labenv_sim_app; eauto.
+      simpl.
+      intros; split; intros; dcr; inv_get; simpl in *; subst; try cases; eauto with len.
+    + pno_step. edestruct H; eauto. len_simpl. inv_get.
+  - pno_step.
+  - pone_step. left.
+    eapply (IH s); eauto with len.
+    rewrite !map_app. intros.
+    eapply labenv_sim_extension_ptw; eauto with len.
+    + intros; hnf; intros; inv_get; eauto.
+      simpl in *; dcr; subst. get_functional.
+      eapply IH; eauto with len. rewrite !map_app; eauto.
+    + hnf; intros; simpl in *; subst; inv_get; simpl; eauto.
+Qed.
+
+Lemma labenv_sim_refl t r L
+  : sawtooth L
+    -> labenv_sim t (sim r) SR (@length _ ⊝ F.block_Z ⊝ L) L L.
+Proof.
+  intros. hnf; dcr; do 4 try split; eauto with len.
+  - intros [] []; intros; simpl in *; subst; inv_get; split; eauto.
+  - split. hnf; intros; simpl in *; inv_get; eauto.
+    hnf; intros; simpl in *. destruct f, f'; simpl in *; subst.
+    get_functional; dcr; subst; inv_get.
+    pone_step; simpl; eauto with len.
+    left. eapply sim_refl.
+Qed.
+
+Lemma labenv_sim_sym L L'
+  : labenv_sim Bisim (sim bot3) SR (@length _ ⊝ F.block_Z ⊝ L') L L'
+    -> labenv_sim Bisim (sim bot3) SR (@length _ ⊝ F.block_Z ⊝ L) L' L.
+Proof.
+  intros []; intros; dcr; do 4 (try split; eauto with len).
+  - hnf; intros. destruct f,f'; simpl in *; subst.
+    exploit (H2 (LabI n0) (LabI n0)); eauto. simpl in *. dcr; subst; eauto.
+    inv_get. eauto.
+  - split.
+    + hnf; intros; simpl in *; inv_get; eauto.
+    + hnf; intros.
+      eapply bisim_sym. simpl in *; dcr; subst.
+      destruct f, f'; simpl in *; subst.
+      eapply H6; eauto. simpl. eauto with len.
+Qed.
+
+
+Lemma bisimeq_sym s1 s2
+  : bisimeq bot3 Bisim s1 s2
+    -> bisimeq bot3 Bisim s2 s1.
+Proof.
+  intros. hnf; intros.
+  eapply bisim_sym. eapply H; eauto.
+  eapply labenv_sim_sym; eauto.
+Qed.
+
+Lemma bisimeq_trans t s1 s2 s3
+  : bisimeq bot3 t s1 s2
+    -> bisimeq bot3 t s2 s3
+    -> bisimeq bot3 t s1 s3.
+Proof.
+  intros. hnf; intros.
+  eapply sim_trans with (S2:=F.state). eauto.
+  eapply H0; eauto.
+  intros. eapply labenv_sim_refl; eauto.
+  eapply H1; eauto.
+Qed.
+
+Lemma labenv_sim_trans t (L1 L2 L3:F.labenv)
+  : labenv_sim t (sim bot3) SR (@length _ ⊝ F.block_Z ⊝ L2) L1 L2
+    -> labenv_sim t (sim bot3) SR (@length _ ⊝ F.block_Z ⊝ L3) L2 L3
+    -> labenv_sim t (sim bot3) SR (@length _ ⊝ F.block_Z ⊝ L3) L1 L3.
+Proof.
+  intros.
+  assert (❬L1❭ = ❬L2❭). {
+    destruct H; dcr. rewrite <- H. eauto with len.
+  }
+  assert (❬L2❭ = ❬L3❭). {
+    destruct H0; dcr. rewrite <- H0. eauto with len.
+  }
+  hnf; dcr; do 4 try split; eauto with len.
+  - destruct H, H0; dcr; eauto.
+  - eapply H.
+  - hnf; intros; simpl in *; destruct f,f'; simpl in *; subst; inv_get.
+    simpl. destruct x.
+    destruct H as [_ [_ [_ [PA1 _]]]]. destruct H0 as [_ [_ [_ [PA2 _]]]].
+    exploit (PA1 (LabI n0) (LabI n0)); eauto; simpl in *; dcr; subst.
+    exploit (PA2 (LabI n0) (LabI n0)); eauto; simpl in *; dcr; subst.
+    split; omega.
+  - split.
+    + hnf; intros; simpl in *; inv_get; eauto.
+    + hnf; intros; simpl in *. destruct f, f'; simpl in *; subst.
+      inv_get; dcr; subst; simpl in *.
+      eapply sim_trans with (S2:=F.state).
+      eapply labenv_sim_app; eauto.
+      Focus 2.
+      eapply labenv_sim_app; eauto.
+      intros; simpl in *; dcr; repeat subst; repeat get_functional.
+      split; intros; eauto with len. cases; split; eauto. congruence.
+      intros; simpl in *; dcr. destruct x; simpl in *.
+      repeat subst; repeat get_functional.
+      split; intros; eauto. eexists; split; eauto. split; eauto with len.
+      split; eauto with len. congruence.
+      cases; eauto. split; intros. congruence.
+      eauto with len.
+Qed.
